

Multiplicative Functions

Theorem : (7.3)

The function d is multiplicative.

Proof. Let m and n be relatively prime. Then, no prime that divides m can divide n and vice versa. Thus, if

$$m = p_1^{e_1} \dots p_k^{e_k} \quad \text{and} \quad n = q_1^{f_1} \dots q_r^{f_r}$$

are the prime power decompositions of m and n , then $p_i \neq q_j$. Then, the prime power decomposition of mn is given by

$$mn = p_1^{e_1} \dots p_k^{e_k} q_1^{f_1} \dots q_r^{f_r}$$

Applying Theorem 7.1, we have that

$$\begin{aligned} d(mn) &= d\left(p_1^{e_1} \dots p_k^{e_k} q_1^{f_1} \dots q_r^{f_r}\right) \\ &= d\left(p_1^{e_1}\right) \dots d\left(p_k^{e_k}\right) d\left(q_1^{f_1}\right) d\left(q_r^{f_r}\right) \\ &= d\left(p_1^{e_1} \dots p_k^{e_k}\right) d\left(q_1^{f_1} \dots q_r^{f_r}\right) \\ &= d(m) d(n) \end{aligned}$$

□

Theorem : (7.4)

The function σ is multiplicative.

Proof. Let m and n be relatively prime. Then, no prime that divides m can divide n and vice versa. Thus, if

$$m = p_1^{e_1} \dots p_k^{e_k} \quad \text{and} \quad n = q_1^{f_1} \dots q_r^{f_r}$$

are the prime power decompositions of m and n , then $p_i \neq q_j$. Then, the prime power decomposition of mn is given by

$$mn = p_1^{e_1} \dots p_k^{e_k} q_1^{f_1} \dots q_r^{f_r}$$

Applying Theorem 7.2, we have that

$$\begin{aligned} \sigma(mn) &= \sigma\left(p_1^{e_1} \dots p_k^{e_k} q_1^{f_1} \dots q_r^{f_r}\right) \\ &= \sigma\left(p_1^{e_1}\right) \dots \sigma\left(p_k^{e_k}\right) \sigma\left(q_1^{f_1}\right) \sigma\left(q_r^{f_r}\right) \\ &= \sigma\left(p_1^{e_1} \dots p_k^{e_k}\right) \sigma\left(q_1^{f_1} \dots q_r^{f_r}\right) \\ &= \sigma(m) \sigma(n) \end{aligned}$$

□

Theorem : (7.5)

If f is a multiplicative function and the prime power decomposition of n is $p_1^{e_1} p_2^{e_2} \dots p_k^{e_k}$, then

$$f(n) = f\left(p_1^{e_1}\right) f\left(p_2^{e_2}\right) \dots f\left(p_k^{e_k}\right)$$

Proof. Base case: $k = 1$: $f(n) = f(p_1^{e_1})$. Assume the theorem is true for $k = r$. Now consider $k = r + 1$. Since $(p_1^{e_1} p_2^{e_2} \dots p_r^{e_r}, p_{r+1}^{e_{r+1}}) = 1$, we have from the definition of a multiplicative function that

$$f(p_1^{e_1} p_2^{e_2} \dots p_r^{e_r} p_{r+1}^{e_{r+1}}) = f(p_1^{e_1} p_2^{e_2} \dots p_r^{e_r}) f(p_{r+1}^{e_{r+1}})$$

From the induction hypothesis, the first factor is

$$f(p_1^{e_1} p_2^{e_2} \dots p_r^{e_r}) = f(p_1^{e_1}) f(p_2^{e_2}) \dots f(p_r^{e_r})$$

Therefore, we have that

$$f(p_1^{e_1} p_2^{e_2} \dots p_r^{e_r} p_{r+1}^{e_{r+1}}) = f(p_1^{e_1}) f(p_2^{e_2}) \dots f(p_r^{e_r}) f(p_{r+1}^{e_{r+1}})$$

□

Perfect Numbers

Definition : Perfect Numbers

A number is called perfect if and only if it is equal to the sum of its positive divisors, excluding itself. That is, a number is perfect if and only if

$$\sigma(n) = 2n$$

Example

Is 6 a perfect number? Is 12 a perfect number?

6 is perfect since $6 = 1 + 2 + 3$.

12 is not perfect since $12 \neq 1 + 2 + 3 + 4 + 6$

Theorem : (8.1) (Euclid)

If $2^k - 1$ is prime, then $2^{k-1} (2^k - 1)$ is perfect.

Proof. Suppose that $n = (2^{k-1}) (2^k - 1)$. Since $2^k - 1$ is prime, we know that

$$\sigma(2^k - 1) = 1 + 2^k - 1 = 2^k$$

Also, notice that 2^{k-1} and $2^k - 1$ are relatively prime. Therefore, n is perfect since

$$\begin{aligned} \sigma(n) &= \sigma(2^{k-1} (2^k - 1)) \\ &= \sigma(2^{k-1}) \sigma(2^k - 1) \\ &= (2^k - 1) 2^k \\ &= 2((2^k - 1) 2^{k-1}) \\ &= 2n \end{aligned}$$

□

Lemma

If k is composite, then $2^k - 1$ is composite.

Proof. Suppose $k = ab$, where $a \neq 1$, $b \neq 1$. Then,

$$\begin{aligned} 2^k - 1 &= 2^{ab} - 1 \\ &= (2^a - 1)(2^{a(b-1)} + 2^{a(b-2)} + \dots + 2^a + 1) \end{aligned}$$

Therefore, 2^{k-1} can be prime only when k is prime. □

Theorem : (8.2) (Euler)

If n is an even perfect number, then

$$n = 2^{p-1} (2^p - 1)$$

for some prime p and $2^p - 1$ is also prime.

Proof. If n is an even perfect number, $n = 2^e m$, where m is odd and $e \geq 1$. Since $\sigma(m) > m$, we can write $\sigma(m) = m + s$, with $s > 0$. That is, s is the sum of all the divisors of m that are less than m . Therefore, substituting this into the expression for $\sigma(n) = 2n$ gives us that

$$\begin{aligned} \sigma(n) &= 2n \\ \sigma(2^e m) &= 2n \\ \sigma(2^e) \sigma(m) &= 2n \\ (2^{e+1} - 1)(m + s) &= 2^{e+1}m \\ 2^{e+1}m - m + (2^{e+1} - 1)s &= 2^{e+1}m \\ (2^{e+1} - 1)s &= m \end{aligned}$$

This means that s is a divisor of m , and $s < m$. But s is the sum of all the divisors of m that are less than m . That is, s is the sum of a group of numbers that includes s . This is only possible if the group consists of one number alone. Therefore the set of divisors of m smaller than m must contain only one element, and that element must be 1. That is, $s = 1$, and hence $m = 2^{e+1} - 1$ is prime. The only numbers of this form that are prime must have $e + 1$ prime. Hence, $m = 2^p - 1$ for some prime $p = e + 1$. Therefore we have

$$\begin{aligned} n &= 2^e m \\ &= 2^e (2^{e+1} - 1) \\ &= 2^{p-1} (2^p - 1) \end{aligned}$$

□